Rewriting for 32-bit DER length, continued

src/lowparse/LowParse.SLow.DER.fst
@@ -12,42 +12,6 @@ module Math = LowParse.Math
 
 #reset-options "--z3cliopt smt.arith.nl=false --max_fuel 0 --max_ifuel 0"
 
-let be_int_of_bounded_integer
-  (len: integer_size)
-  (x: nat { x < pow2 (8 * len) } )
-: GTot (bounded_integer len)
-= integer_size_values len;
-  assert_norm (pow2 (8 * 1) == 256);
-  assert_norm (pow2 (8 * 2) == 65536);
-  assert_norm (pow2 (8 * 3) == 16777216);
-  assert_norm (pow2 (8 * 4) == 4294967296);
-  U32.uint_to_t x
-
-let be_int_of_bounded_integer_injective
-  (len: integer_size)
-: Lemma
-  (synth_injective (be_int_of_bounded_integer len))
-  [SMTPat (synth_injective (be_int_of_bounded_integer len))] // FIXME: WHY WHY WHY does this pattern NEVER trigger?
-= integer_size_values len;
-  assert_norm (pow2 (8 * 1) == 256);
-  assert_norm (pow2 (8 * 2) == 65536);
-  assert_norm (pow2 (8 * 3) == 16777216);
-  assert_norm (pow2 (8 * 4) == 4294967296)
-
-let parse_seq_flbytes_synth_be_int_eq
-  (len: integer_size)
-  (input: bytes)
-: Lemma
-  (
-    let _ = synth_be_int_injective len in
-    let _ = be_int_of_bounded_integer_injective len in
-    parse ((parse_seq_flbytes len `parse_synth` synth_be_int len) `parse_synth` be_int_of_bounded_integer len) input == parse (parse_bounded_integer len) input)
-=
-    let _ = synth_be_int_injective len in
-    let _ = be_int_of_bounded_integer_injective len in
-    parse_synth_eq (parse_seq_flbytes len `parse_synth` synth_be_int len) (be_int_of_bounded_integer len) input;
-    parse_synth_eq (parse_seq_flbytes len) (synth_be_int len) input
-
 
 (*
 inline_for_extraction
